alternative finito

Lean/basic.lean
@@ -58,40 +58,40 @@ by { induction f; simp [*, max_comm] }
 prefix `↓` : 70 := int.to_nat
 
 def ev : RPP → list ℤ → list ℤ
-| (Id n)     l                    := l
-| Ne         (x :: l)             := -x :: l
-| Su         (x :: l)             := (x + 1) :: l
-| Pr         (x :: l)             := (x - 1) :: l
-| Sw         (x :: y :: l)        := y :: x :: l
-| (f ;; g)   l                    := ev g (ev f l)
-| (f ‖ g)    l                    := ev f (take f.arity l) ++ ev g (drop f.arity l)
-| (It f)     (x :: l)             := x :: ((ev f)^[↓x] l)
-| (If f g h) (0 :: l)             := 0 :: ev g l
-| (If f g h) (((n : ℕ) + 1) :: l) := (n + 1) :: ev f l
-| (If f g h) (-[1+ n] :: l)       := -[1+ n] :: ev h l
-| _          l                    := l
+| (Id n)     X                    := X
+| Ne         (x :: X)             := -x :: X
+| Su         (x :: X)             := (x + 1) :: X
+| Pr         (x :: X)             := (x - 1) :: X
+| Sw         (x :: y :: X)        := y :: x :: X
+| (f ;; g)   X                    := ev g (ev f X)
+| (f ‖ g)    X                    := ev f (take f.arity X) ++ ev g (drop f.arity X)
+| (It f)     (x :: X)             := x :: ((ev f)^[↓x] X)
+| (If f g h) (0 :: X)             := 0 :: ev g X
+| (If f g h) (((n : ℕ) + 1) :: X) := (n + 1) :: ev f X
+| (If f g h) (-[1+ n] :: X)       := -[1+ n] :: ev h X
+| _          X                    := X
 
 notation `‹` f `›` : 50 := ev f -- ‹ \f › \fr
 
 @[simp] lemma ev_nil (f : RPP) : ‹f› [] = [] :=
 by { induction f; simp [ev, *] }
 
-@[simp] lemma ev_length (f : RPP) (l : list ℤ) : (‹f› l).length = l.length :=
+@[simp] lemma ev_length (f : RPP) (X : list ℤ) : (‹f› X).length = X.length :=
 begin
-  induction f generalizing l; cases l with x l,
+  induction f generalizing X; cases X with x X,
   any_goals {simp [ev, *], done},
-  { cases l with x l; refl },
+  { cases X with x X; refl },
   { simp [ev], rw [f_ih_f, f_ih_g, ←length_append, take_append_drop], refl },
   { simp [ev], induction (↓x), refl, rw [function.iterate_succ_apply'], simp * },
   { cases x, cases x, all_goals {simp [ev, *]} }
 end
 
-lemma pa_co_pa (f f' g g' : RPP) (l : list ℤ) : f.arity = f'.arity →
-  ‹f ‖ g ;; f' ‖ g'› l = ‹(f ;; f') ‖ (g ;; g')› l :=
+lemma pa_co_pa (f f' g g' : RPP) (X : list ℤ) : f.arity = f'.arity →
+  ‹f ‖ g ;; f' ‖ g'› X = ‹(f ;; f') ‖ (g ;; g')› X :=
 begin
   intro h,
   simp [ev], rw [←h, max_self], clear h,
-  cases (le_total f.arity l.length) with H H,
+  cases (le_total f.arity X.length) with H H,
   { rw [take_append_of_le_length, drop_append_of_le_length],
     rw [take_all_of_le, drop_eq_nil_of_le],
     refl, all_goals {simp *} },
@@ -100,35 +100,35 @@ begin
     all_goals {simp *} }
 end
 
-theorem inv_co_l (f : RPP) (l : list ℤ) : ‹f ;; f⁻¹› l = l :=
+theorem inv_co_l (f : RPP) (X : list ℤ) : ‹f ;; f⁻¹› X = X :=
 begin
-  induction f generalizing l; cases l with x l,
+  induction f generalizing X; cases X with x X,
   any_goals {simp [ev, *], done},
-  { cases l with y l, refl, simp [ev] },
+  { cases X with y X, refl, simp [ev] },
   { simp [ev, *] at * },
   { rw [inv, pa_co_pa], simp [ev, *] at *, rw arity_inv },
   { simp [ev] at *, apply function.left_inverse.iterate f_ih },
   { rcases x with ⟨n, n⟩; simp [ev, *] at * }
 end
 
-lemma inv_co_r (f : RPP) (l : list ℤ) : ‹f⁻¹ ;; f› l = l :=
-by { convert inv_co_l (f⁻¹) l, rw inv_involute }
+lemma inv_co_r (f : RPP) (X : list ℤ) : ‹f⁻¹ ;; f› X = X :=
+by { convert inv_co_l (f⁻¹) X, rw inv_involute }
 
-@[simp] theorem inv_iff (f : RPP) (l m : list ℤ) : ‹f⁻¹› l = m ↔ ‹f› m = l :=
+@[simp] theorem inv_iff (f : RPP) (X Y : list ℤ) : ‹f⁻¹› X = Y ↔ ‹f› Y = X :=
 begin
   split; intro h; rw ←h,
-  conv_rhs {rw ←inv_co_r f l}, refl,
-  conv_rhs {rw ←inv_co_l f m}, refl,
+  conv_rhs {rw ←inv_co_r f X}, refl,
+  conv_rhs {rw ←inv_co_l f Y}, refl,
 end
 
-lemma take_ev (f : RPP) (n : ℕ) (l : list ℤ) : f.arity ≤ n →
-  take n (‹f› l) = ‹f› (take n l) :=
+lemma take_ev (f : RPP) (n : ℕ) (X : list ℤ) : f.arity ≤ n →
+  take n (‹f› X) = ‹f› (take n X) :=
 begin
   intro h,
-  induction f generalizing n l,
-  any_goals { cases l; cases n; refl },
+  induction f generalizing n X,
+  any_goals { cases X; cases n; refl },
   { rw arity at h, rcases n with _ | _ | n, linarith, linarith,
-    rcases l with _ | ⟨x, _ | l⟩; refl },
+    rcases X with _ | ⟨x, _ | l⟩; refl },
   { rw [arity, max_le_iff] at h, cases h with h₁ h₂, simp [ev, *] },
   case Pa : f g hf hg
   { rw arity at h,
@@ -139,30 +139,30 @@ begin
     rw [take_take, min_eq_right h₁],
     rw [take_take, min_eq_left h₁],
     rw [ev_length, length_take],
-    cases (le_total f.arity l.length) with H H,
+    cases (le_total f.arity X.length) with H H,
     rw [min_eq_left H, hg, ←drop_take], congr, omega, omega,
     rw [drop_eq_nil_of_le H, drop_eq_nil_of_le, take_all_of_le]; simp * },
   case It : f hf
-  { cases l with x l; cases n; try {refl},
+  { cases X with x X; cases n; try {refl},
     simp [ev],
-    induction (↓x) generalizing l, refl,
+    induction (↓x) generalizing X, refl,
     replace h := nat.succ_le_succ_iff.mp h,
     simp [arity, *] at * },
-  { cases l with x l; cases n; try {refl},
+  { cases X with x X; cases n; try {refl},
     rw arity at h, replace h := nat.succ_le_succ_iff.mp h, simp [max_le_iff] at h, 
     rcases h with ⟨⟨h₁, h₂⟩, h₃⟩,
     cases x, cases x, all_goals {simp [ev, *]} }
 end
 
-lemma drop_ev (f : RPP) (n : ℕ) (l : list ℤ) : f.arity ≤ n →
-  drop n (‹f› l) = drop n l :=
+lemma drop_ev (f : RPP) (n : ℕ) (X : list ℤ) : f.arity ≤ n →
+  drop n (‹f› X) = drop n X :=
 begin
   intro h,
-  induction f generalizing n l,
+  induction f generalizing n X,
   { refl },
-  any_goals { rw arity at h, cases n, linarith, cases l; refl },
+  any_goals { rw arity at h, cases n, linarith, cases X; refl },
   { rw arity at h, rcases n with _ | _ | n, linarith, linarith,
-    rcases l with _ | ⟨x, _ | l⟩; refl },
+    rcases X with _ | ⟨x, _ | l⟩; refl },
   { rw [arity, max_le_iff] at h, cases h with h₁ h₂, simp [ev, *] },
   case Pa : f g hf hg
   { rw arity at h,
@@ -172,28 +172,28 @@ begin
     rw [drop_append_eq_append_drop, hf _ _ h₁],
     rw [drop_eq_nil_of_le, nil_append],
     rw [ev_length, length_take ],
-    cases (le_total f.arity l.length) with H H,
+    cases (le_total f.arity X.length) with H H,
     rw [min_eq_left H, hg, drop_drop], congr, omega, omega,
     rw [drop_eq_nil_of_le H, ev_nil, drop_nil, drop_eq_nil_of_le], linarith, simp * },
   case It : f hf
-  { cases n, rw arity at h, linarith, cases l with x l, refl,
+  { cases n, rw arity at h, linarith, cases X with x X, refl,
     rw [ev, drop],
-    induction (↓x) generalizing l, refl,
+    induction (↓x) generalizing X, refl,
     replace h := nat.succ_le_succ_iff.mp h, simp [arity, *] at * },
-  { cases n, rw arity at h, linarith, cases l with x l, refl,
+  { cases n, rw arity at h, linarith, cases X with x X, refl,
     rw arity at h, replace h := nat.succ_le_succ_iff.mp h, simp [max_le_iff] at h, 
     rcases h with ⟨⟨h₁, h₂⟩, h₃⟩,
     cases x, cases x, all_goals {simp [ev, *]} }
 end
 
-theorem ev_split (f : RPP) (l : list ℤ) :
-  ‹f› l = ‹f› (take f.arity l) ++ drop f.arity l :=
+theorem ev_split (f : RPP) (X : list ℤ) :
+  ‹f› X = ‹f› (take f.arity X) ++ drop f.arity X :=
 begin
   rw [←take_ev, ←drop_ev, take_append_drop], refl, refl 
 end
 
-lemma ev_split_le (f : RPP) (l : list ℤ) (n : ℕ) : f.arity ≤ n →
-  ‹f› l = ‹f› (take n l) ++ drop n l :=
+lemma ev_split_le (f : RPP) (X : list ℤ) (n : ℕ) : f.arity ≤ n →
+  ‹f› X = ‹f› (take n X) ++ drop n X :=
 begin
   intro h, rw [←take_ev, ←drop_ev, take_append_drop], assumption, assumption
 end
