Lean/prf_complete.lean
@@ -1,19 +1,19 @@
 import pair
 
-def nat.prec_loop (F G : ℕ → ℕ) (z n : ℕ) :=
+def nat.prec (F G : ℕ → ℕ) (z n : ℕ) :=
   nat.elim (F z) (λ (y IH : ℕ), G (nat.mkpair z (nat.mkpair y IH))) n
 
 open list
 
 namespace RPP
 
-def ex_rpp (F : ℕ → ℕ) (f : RPP) :=
+def encode (F : ℕ → ℕ) (f : RPP) :=
   ∀ (z : ℤ) (n : ℕ), ‹f› (z :: n :: repeat 0 (f.arity-2)) = (z + F n) :: n :: repeat 0 (f.arity-2)
 
-lemma ex_rpp_le (F : ℕ → ℕ) (f : RPP) : ex_rpp F f → ∀ (a : ℕ), f.arity-2 ≤ a →
+lemma encode_le (F : ℕ → ℕ) (f : RPP) : encode F f → ∀ (a : ℕ), f.arity-2 ≤ a →
   ∀ (z : ℤ) (n : ℕ), ‹f› (z :: n :: repeat 0 a) = (z + F n) :: n :: repeat 0 a :=
 begin
-  rw ex_rpp, intros H a h z n,
+  rw encode, intros H a h z n,
   cases (le_total f.arity 2) with h₁,
 
   have h₂ : f.arity-2 = 0, from sub_eq_zero_iff_le.mpr h₁,
@@ -84,14 +84,14 @@ begin
 end
 
 lemma pair_fwd_def (F G : ℕ → ℕ) (f g : RPP) :
-  ex_rpp F f → ex_rpp G g → ∀ (z : ℤ) (n : ℕ),
+  encode F f → encode G g → ∀ (z : ℤ) (n : ℕ),
   ‹pair_fwd f g› (z :: n :: repeat 0 ((pair_fwd f g).arity-2)) =
   nat.mkpair (F n) (G n) :: z :: n :: F n :: G n :: 0 :: repeat 0 ((pair_fwd f g).arity-6) :=
 begin
   intros hF hG z n,
   rcases pair_fwd_arity f g with ⟨a, h₁, h₂, h₃⟩, rw h₁,
-  have HF := ex_rpp_le _ _ hF _ h₂, clear hF,
-  have HG := ex_rpp_le _ _ hG _ h₃, clear hG,
+  have HF := encode_le _ _ hF _ h₂, clear hF,
+  have HG := encode_le _ _ hG _ h₃, clear hG,
   simp [pair_fwd, ev, rewire, *] at *
 end
 
@@ -103,7 +103,7 @@ begin
   have h := pair_fwd_arity_le1 f g, linarith
 end
 
-lemma pair_def (F G : ℕ → ℕ) (f g : RPP) : ex_rpp F f → ex_rpp G g → ∀ (z : ℤ) (n : ℕ),
+lemma pair_def (F G : ℕ → ℕ) (f g : RPP) : encode F f → encode G g → ∀ (z : ℤ) (n : ℕ),
   ‹pair f g› (z :: n :: repeat 0 ((pair f g).arity-2)) =
   (z + nat.mkpair (F n) (G n)) :: n :: repeat 0 ((pair f g).arity-2) :=
 begin
@@ -148,14 +148,14 @@ begin
   split, omega, omega
 end
 
-lemma comp_fwd_def (F G : ℕ → ℕ) (f g : RPP) : ex_rpp F f → ex_rpp G g → ∀ (z : ℤ) (n : ℕ),
+lemma comp_fwd_def (F G : ℕ → ℕ) (f g : RPP) : encode F f → encode G g → ∀ (z : ℤ) (n : ℕ),
   ‹comp_fwd f g› (z :: n :: repeat 0 ((comp_fwd f g).arity-2)) =
   F (G n) :: z :: n :: ↑(G n) :: repeat 0 ((comp_fwd f g).arity-4) :=
 begin
   intros hF hG z n,
   rcases comp_fwd_arity f g with ⟨a, h₁, h₂, h₃⟩, rw h₁,
-  have HF := ex_rpp_le _ _ hF _ h₂, clear hF,
-  have HG := ex_rpp_le _ _ hG _ h₃, clear hG,
+  have HF := encode_le _ _ hF _ h₂, clear hF,
+  have HG := encode_le _ _ hG _ h₃, clear hG,
   simp [comp_fwd, ev, rewire, *] at *
 end
 
@@ -167,7 +167,7 @@ begin
   have h := comp_fwd_arity_le1 f g, linarith
 end
 
-lemma comp_def (F G : ℕ → ℕ) (f g : RPP) : ex_rpp F f → ex_rpp G g → ∀ (z : ℤ) (n : ℕ),
+lemma comp_def (F G : ℕ → ℕ) (f g : RPP) : encode F f → encode G g → ∀ (z : ℤ) (n : ℕ),
   ‹comp f g› (z :: n :: repeat 0 ((comp f g).arity-2)) =
   (z + F (G n)) :: n :: repeat 0 ((comp f g).arity-2) :=
 begin
@@ -176,7 +176,7 @@ begin
   simp [comp, ev, *]
 end
 
-def prec_loop (g : RPP) :=
+def prec_step (g : RPP) :=
   Id 2 ‖ mkpair ;;
   Id 1 ‖ mkpair ;;
   Id 1 ‖ (Sw ;; g) ;;
@@ -191,24 +191,24 @@ def prec_fwd (f g : RPP) :=
   ⌊0, 2, 3, 1⌉ ;;
   Id 2 ‖ f ;;
   ⌊0, 1, 4, 3, 5, 2⌉ ;;
-  Id 1 ‖ It (prec_loop g) ;;
+  Id 1 ‖ It (prec_step g) ;;
   ⌊5, 0⌉
 
 lemma prec_fwd_arity_le1 (f g : RPP) : 12 ≤ (prec_fwd f g).arity :=
 begin
-  rw [prec_fwd, prec_loop], simp,
+  rw [prec_fwd, prec_step], simp,
   left, right, rw [show 12 = 1 + (10 + 1), by refl], simp
 end
 
 lemma prec_fwd_arity_le2 (f g : RPP) : f.arity + 2 ≤ (prec_fwd f g).arity :=
 begin
-  rw [prec_fwd, prec_loop], simp,
+  rw [prec_fwd, prec_step], simp,
   left, left, left, right, rw add_comm
 end
 
 lemma prec_fwd_arity_le3 (f g : RPP) : g.arity + 3 ≤ (prec_fwd f g).arity :=
 begin
-  rw [prec_fwd, prec_loop], simp,
+  rw [prec_fwd, prec_step], simp,
   left, right, rw [show g.arity + 3 = 1 + (g.arity + 1 + 1), by ring], simp,
   left, left, left, right,
   rw [add_comm, add_le_add_iff_left],
@@ -226,38 +226,38 @@ begin
   split, omega, omega
 end
 
-lemma prec_loop_def (F G : ℕ → ℕ) (f g : RPP) : ex_rpp G g → ∀ (Z N s : ℕ), ∃ (s' : ℕ),
-  ‹prec_loop g› (s :: Z :: N :: nat.prec_loop F G Z N :: repeat 0 ((prec_fwd f g).arity-6)) =
-  s' :: Z :: (N + 1) :: nat.prec_loop F G Z (N + 1) :: repeat 0 ((prec_fwd f g).arity-6) :=
+lemma prec_step_def (F G : ℕ → ℕ) (f g : RPP) : encode G g → ∀ (z n s : ℕ), ∃ (s' : ℕ),
+  ‹prec_step g› (s :: z :: n :: nat.prec F G z n :: repeat 0 ((prec_fwd f g).arity-6)) =
+  s' :: z :: (n + 1) :: nat.prec F G z (n + 1) :: repeat 0 ((prec_fwd f g).arity-6) :=
 begin
-  intros hG Z N s, use nat.mkpair s (nat.prec_loop F G Z N),
+  intros hG z n s, use nat.mkpair s (nat.prec F G z n),
   rcases prec_fwd_arity f g with ⟨a, h₁, h₂, h₃⟩, rw h₁,
-  have HG := ex_rpp_le _ _ hG _ h₃, clear hG,
-  simp [prec_loop, nat.prec_loop, ev, rewire, *] at *
+  have HG := encode_le _ _ hG _ h₃, clear hG,
+  simp [prec_step, nat.prec, ev, rewire, *] at *
 end
 
-lemma it_prec_loop_def (F G : ℕ → ℕ) (f g : RPP) : ex_rpp G g → ∀ (Z N : ℕ), ∃ (s : ℕ),
-  ‹prec_loop g›^[N] (0 :: Z :: 0 :: F Z :: repeat 0 ((prec_fwd f g).arity-6)) =
-  s :: Z :: N :: nat.prec_loop F G Z N :: repeat 0 ((prec_fwd f g).arity-6) :=
+lemma it_prec_step_def (F G : ℕ → ℕ) (f g : RPP) : encode G g → ∀ (z n : ℕ), ∃ (s : ℕ),
+  ‹prec_step g›^[n] (0 :: z :: 0 :: F z :: repeat 0 ((prec_fwd f g).arity-6)) =
+  s :: z :: n :: nat.prec F G z n :: repeat 0 ((prec_fwd f g).arity-6) :=
 begin
-  intros hG Z N, induction N with N hN,
+  intros hG z n, induction n with n hN,
   use 0, simp [ev], refl,
   rcases hN with ⟨s, hN⟩,
-  have h := prec_loop_def F G f g hG Z N s, rcases h with ⟨s', h⟩,
+  have h := prec_step_def F G f g hG z n s, rcases h with ⟨s', h⟩,
   use s', rw [function.iterate_succ_apply', hN, h], refl
 end
 
 lemma prec_fwd_def (F G : ℕ → ℕ) (f g : RPP) :
-  ex_rpp F f → ex_rpp G g → ∀ (n : ℕ), ∃ (s : ℕ), ∀ (z : ℤ),
+  encode F f → encode G g → ∀ (n : ℕ), ∃ (s : ℕ), ∀ (z : ℤ),
   ‹prec_fwd f g› (z :: n :: repeat 0 ((prec_fwd f g).arity-2)) =
-  nat.prec_loop F G (nat.unpair n).fst (nat.unpair n).snd ::
+  nat.prec F G (nat.unpair n).fst (nat.unpair n).snd ::
     z :: (nat.unpair n).snd :: s :: (nat.unpair n).fst :: (nat.unpair n).snd ::
     repeat 0 ((prec_fwd f g).arity-6) :=
 begin
   intros hF hG n,
   rcases prec_fwd_arity f g with ⟨a, h₁, h₂, h₃⟩, rw h₁ at *,
-  have HF := ex_rpp_le _ _ hF _ h₂, clear hF,
-  have h := it_prec_loop_def F G f g hG (nat.unpair n).fst (nat.unpair n).snd,
+  have HF := encode_le _ _ hF _ h₂, clear hF,
+  have h := it_prec_step_def F G f g hG (nat.unpair n).fst (nat.unpair n).snd,
   rcases h with ⟨s, h⟩, use s, intro z,
   simp [prec_fwd, ev, rewire, *] at *
 end
@@ -270,9 +270,9 @@ begin
   have h := prec_fwd_arity_le1 f g, linarith
 end
 
-lemma prec_def (F G : ℕ → ℕ) (f g : RPP) : ex_rpp F f → ex_rpp G g → ∀ (z : ℤ) (n : ℕ),
+lemma prec_def (F G : ℕ → ℕ) (f g : RPP) : encode F f → encode G g → ∀ (z : ℤ) (n : ℕ),
   ‹prec f g› (z :: n :: repeat 0 ((prec f g).arity-2)) =
-  (z + nat.prec_loop F G (nat.unpair n).fst (nat.unpair n).snd) ::
+  (z + nat.prec F G (nat.unpair n).fst (nat.unpair n).snd) ::
     n :: repeat 0 ((prec f g).arity-2) :=
 begin
   intros hF hG z n, rw prec_arity_eq,
@@ -280,22 +280,22 @@ begin
   simp [prec, ev, *]
 end
 
-theorem completeness (F : ℕ → ℕ) : nat.primrec F → ∃ f, ex_rpp F f :=
+theorem completeness (F : ℕ → ℕ) : nat.primrec F → ∃ f, encode F f :=
 begin
   intro h, induction h,
-  case zero : { use Id 0, simp [ex_rpp, ev] },
+  case zero : { use Id 2, simp [encode, ev] },
   case succ : { use succ, exact succ_def },
   case left : { use left, exact left_def },
   case right : { use right, exact right_def },
   case pair : G₁ G₂ h₁ h₂ ih₁ ih₂
   { rcases ih₁ with ⟨g₁, ih₁⟩, rcases ih₂ with ⟨g₂, ih₂⟩,
-    use pair g₁ g₂, rw ex_rpp, exact pair_def _ _ _ _ ih₁ ih₂ },
+    use pair g₁ g₂, rw encode, exact pair_def _ _ _ _ ih₁ ih₂ },
   case comp : G₁ G₂ h₁ h₂ ih₁ ih₂
   { rcases ih₁ with ⟨g₁, ih₁⟩, rcases ih₂ with ⟨g₂, ih₂⟩,
-    use comp g₁ g₂, rw ex_rpp, exact comp_def _ _ _ _ ih₁ ih₂ },
+    use comp g₁ g₂, rw encode, exact comp_def _ _ _ _ ih₁ ih₂ },
   case prec : G₁ G₂ h₁ h₂ ih₁ ih₂
   { rcases ih₁ with ⟨g₁, ih₁⟩, rcases ih₂ with ⟨g₂, ih₂⟩,
-    use prec g₁ g₂, rw ex_rpp, exact prec_def _ _ _ _ ih₁ ih₂ }
+    use prec g₁ g₂, rw encode, exact prec_def _ _ _ _ ih₁ ih₂ }
 end
 
 end RPP
